more

Ordered_Resolution_Prover/Executable_Subsumption.thy
@@ -12,6 +12,44 @@ theory Executable_Subsumption
     "$ISAFOR/Rewriting/Matching"
 begin
 
+definition "ext_gsubst x = Fun (Inr x) []"
+definition "ext_emb = map_term Inl id"
+
+fun undo_ext where
+  "undo_ext (Var x) = Var x"
+| "undo_ext (Fun (Inr x) ts) = Var x"
+| "undo_ext (Fun (Inl x) ts) = Fun x (map undo_ext ts)"
+
+lemma undo_ext_gsubst_inverse[simp]:
+  "undo_ext (ext_gsubst x) = Var x"
+  "undo_ext (ext_emb t \<cdot> \<sigma>) = t \<cdot> (undo_ext o \<sigma>)"
+  "undo_ext (ext_emb t) = t"
+  by (induct t) (auto simp: ext_gsubst_def ext_emb_def cong: map_cong)
+
+lemma subst_ext_gsubst: "t \<cdot> ext_gsubst \<cdot> \<sigma> = t \<cdot> ext_gsubst"
+  by (induct t) (auto simp: ext_gsubst_def)
+
+lemma is_ground_subst_ext_gsubst: "is_ground_subst ext_gsubst"
+  unfolding is_ground_subst_def ext_gsubst_def is_ground_atm_def subst_ext_gsubst by blast
+
+lemma ext_emb_subst[simp]: "ext_emb (t \<cdot> \<sigma>) = ext_emb t \<cdot> (ext_emb o \<sigma>)"
+  by (induct t) (auto simp: ext_emb_def)
+
+lemma subsumes_ground:
+  "subsumes (map_clause ext_emb C) (map_clause ext_emb D \<cdot>cls ext_gsubst) \<longleftrightarrow> subsumes C D"
+  (is "?L \<longleftrightarrow> ?R")
+proof
+  assume ?R
+  then obtain \<sigma> where "subst_cls C \<sigma> \<subseteq># D"
+    unfolding subsumes_def by auto
+  from image_mset_subseteq_mono[of _ _ "map_literal ((\<lambda>t. t \<cdot> ext_gsubst) o ext_emb)", OF this]
+  show ?L
+    by (auto simp: subsumes_def multiset.map_comp literal.map_comp
+     subst_cls_def subst_apply_clause_def subst_lit_def o_def subst_subst subst_compose_def)
+qed (auto simp: subsumes_def multiset.map_comp literal.map_ident literal.map_comp
+     subst_cls_def subst_apply_clause_def subst_lit_def o_def
+     dest!: image_mset_subseteq_mono[of _ _ "map_literal undo_ext"])
+
 context notes length_remove1[termination_simp] find_Some_iff[termination_simp] begin
 fun subsumes_list where
   "subsumes_list [] Ks = Some Var"
@@ -28,43 +66,82 @@ end
 declare subsumes_list.simps(2)[simp del]
 
 lemma atm_of_map_literal[simp]: "atm_of (map_literal f l) = f (atm_of l)"
-  by (cases l) auto
+
+abbreviation subsumes_list_subst  (infixl "\<triangleleft>" 60) where
+  "subsumes_list_subst Ls Ks \<equiv> subsumes (mset Ls) (mset Ks)"
+term match_term_list
+lemma "\<forall>K \<in> set Ks. is_ground_lit K \<Longrightarrow>
+  L # Ls \<triangleleft> Ks \<longleftrightarrow> (\<exists>K \<in> set Ks. \<exists>\<rho>. L \<cdot>lit \<rho> = K \<and> map (\<lambda>L. L \<cdot>lit \<rho>) Ls \<triangleleft> remove1 K Ks)"
+  unfolding subsumes_def
+  apply safe
+  apply (auto simp: insert_subset_eq_iff subst_lit_def subst_cls_def literal.map_ident) []
+   apply (erule bexI[rotated])
+   apply (rule exI conjI)+
+    apply (rule refl)
+   apply (rule exI[of _ Var])
+   apply (auto simp: subst_cls_def subst_lit_def literal.map_ident) []
+  apply (rule_tac x = "\<rho> \<circ>\<^sub>s \<sigma>" in exI)
+  apply (auto simp: insert_subset_eq_iff subst_lit_def subst_cls_def
+    cong: literal.map_cong split: if_splits)
+  
+  find_theorems "add_mset _ _ \<subseteq># _"
+  sorry
 
 lemma subsumes_list_complete:
-  "subsumes_list Ls Ks = None \<Longrightarrow> \<forall>\<rho>. \<not> mset (map (\<lambda>L. L \<cdot>lit \<rho>) Ls) \<subseteq># mset Ks"
-proof (induction Ls Ks rule: subsumes_list.induct[case_names Nil Cons])
+  "subsumes_list Ls Ks = None \<Longrightarrow> \<not> Ls \<triangleleft> Ks"
+  sorry
+proof (induction Ls Ks rule: subsumes_list.induct[case_names Nil_Nil Cons_Nil Cons])
   case (Cons L Ls Ks)
-  from Cons.prems show ?case
-  proof (cases "find (\<lambda>K. is_pos K = is_pos L \<and> match (atm_of K) (atm_of L) \<noteq> None) Ks")
-    case None
-    then show ?thesis
-      apply (auto simp: find_None_iff dest!: spec[of _ "L \<cdot>lit _"] match_complete) sorry
-  next
-    case (Some K)
-    let ?\<rho> = "the (match (atm_of K) (atm_of L))"
-    let ?Ks = "remove1 K Ks"
-    from Cons.prems Some show ?thesis
-    proof (cases "subsumes_list (map (\<lambda>L. L \<cdot>lit ?\<rho>) Ls) ?Ks")
+  show ?case sorry(*
+  proof
+    fix \<rho>
+    from Cons.prems show "\<not> mset (map (\<lambda>a. a \<cdot>lit \<rho>) (L # Ls)) \<subseteq># mset Ks"
+    proof (cases "find (\<lambda>K. is_pos K = is_pos L \<and> match (atm_of K) (atm_of L) \<noteq> None) Ks")
       case None
-      note IH = Cons.IH(1)[OF Some refl refl None]
       then show ?thesis
-        apply (auto simp: image_image literal.map_comp o_def elim!: meta_mp)
+        by (auto simp: find_None_iff dest!: spec[of _ "L \<cdot>lit \<rho>"] match_complete)
+    next
+      case (Some K)
+      let ?\<rho>KL = "the (match (atm_of K) (atm_of L))"
+      let ?Ks = "remove1 K Ks"
+      from Cons.prems Some show ?thesis
+      proof (cases "subsumes_list (map (\<lambda>L. L \<cdot>lit ?\<rho>KL) Ls) ?Ks")
+        case None
+        with Cons.prems Some have "subsumes_list (L # Ls) ?Ks = None"
+          by (subst (asm) subsumes_list.simps(2)) (auto simp: Let_def)
+        note IH =
+          Cons.IH(1)[OF Some refl refl None, THEN spec, of \<rho>]
+          Cons.IH(2)[OF Some refl refl None this, THEN spec, of \<rho>]
+        with Some None show ?thesis
+          apply (auto simp: literal.map_comp o_def insert_subset_eq_iff is_pos_def
+            find_Some_iff subst_subst simp del: subst_subst_compose dest!: match_sound spec[of _ "\<rho>"])
+          sledgehammer
+          subgoal for i \<sigma> t
+           apply (drule spec[of _ "\<rho>"])
+            apply (erule notE)
+            apply auto
+          find_theorems "add_mset _ _ \<subseteq># _"
+          sorry
         sorry
-    qed (subst (asm) subsumes_list.simps(2), auto)
-  qed
+      qed (subst (asm) subsumes_list.simps(2), auto)
+    qed
+  qed*)
 qed simp
 
 lemma subsumes_list_sound:
   "subsumes_list Ls Ks = Some \<rho> \<Longrightarrow> mset (map (\<lambda>L. L \<cdot>lit \<rho>) Ls) \<subseteq># mset Ks"
+  sorry
+(*
 proof (induct Ls Ks arbitrary: \<rho> rule: subsumes_list.induct[case_names Nil Cons])
   case (Cons L Ls Ks)
   then show ?case sorry
 qed simp
+*)
 
 lemma subsumes_subsumes_list[code_unfold]:
   "subsumes (mset Ls) (mset Ks) = (subsumes_list Ls Ks \<noteq> None)"
-  unfolding subsumes_def using subsumes_list_sound[of Ls Ks] subsumes_list_complete[of Ls Ks]
-  by (auto simp: subst_cls_def subst_lit_def)
+  using subsumes_list_sound[of Ls Ks] subsumes_list_complete[of Ls Ks]
+  by (auto simp: subst_cls_def subst_lit_def subsumes_def)
 
 lemma subsumes_list_subsumes:
   "(\<exists>\<sigma>. subsumes_list Ls Ks = Some \<sigma>) = subsumes (mset Ls) (mset Ks)"
